theories/imp_heap_bij_own.v
@@ -1,0 +1,1045 @@
+Require Export iris.algebra.cmra.
+Require Export iris.algebra.lib.gmap_view.
+Require Export refframe.module.
+Require Import refframe.trefines.
+Require Import refframe.filter.
+Require Import refframe.product.
+Require Import refframe.seq_product.
+Require Import refframe.link.
+Require Import refframe.prepost.
+Require Import refframe.proof_techniques.
+Require Import refframe.imp.
+
+Set Default Proof Using "Type".
+
+Section updates.
+  Context {A : cmra}.
+  Lemma cmra_update_included (x y : A) :
+    x ≼ y → y ~~> x.
+  Proof. move => [? ->]. apply cmra_update_op_l. Qed.
+End updates.
+
+Section total_updates.
+  Local Set Default Proof Using "Type*".
+  Context {A : ucmra}.
+  Context `{CmraTotal A} `{CmraDiscrete A}.
+  Lemma ucmra_discrete_update_valid (x y : A) :
+    x ~~> y → ✓ x → ✓ y.
+  Proof.
+    move => /cmra_discrete_update Hv. have := (Hv (@ε A (ucmra_unit A))).
+    rewrite comm left_id comm left_id. naive_solver.
+  Qed.
+End total_updates.
+
+Section included.
+  Context {A : cmra}.
+  Implicit Types (x y z : A).
+  Lemma cmra_included_op_l x y z : x ≼ y → x ≼ y ⋅ z.
+  Proof. intros ?. etrans; [done|]. apply cmra_included_l. Qed.
+  Lemma cmra_included_op_r x y z : x ≼ y → x ≼ z ⋅ y.
+  Proof. intros ?. etrans; [done|]. apply cmra_included_r. Qed.
+End included.
+
+
+Section prepost.
+Context {R : Type} {A : cmra}.
+
+Definition pp_update (P x : A) (pp : A → prepost R) : prepost R :=
+  pp_quant $ λ y,
+  pp_prop (x ~~> P ⋅ y) $
+  pp y.
+
+Definition pp_own (P x : A) (pp : A → prepost R) : prepost R :=
+  pp_prop (✓ (P ⋅ x)) $
+  pp (P ⋅ x).
+End prepost.
+
+
+(** * camera definition *)
+Inductive heap_bij_elem :=
+| HBShared (p : prov) | HBConstant (h : Z → option val) | HBChanging.
+Canonical Structure heap_bij_elemO := leibnizO heap_bij_elem.
+
+Definition heap_bijUR : cmra := gmap_viewUR prov heap_bij_elemO.
+(* Eval simpl in cmra_car heap_bijR. *)
+
+(** * imp_heap_bij_own *)
+Record heap_bij := HeapBij {
+  hb_bij : gmap prov heap_bij_elem;
+  hb_iff p1 p2 p1' p2' :
+   hb_bij !! p2 = Some (HBShared p1) →
+   hb_bij !! p2' = Some (HBShared p1') →
+   p1 = p1' ↔ p2 = p2'
+}.
+
+Global Program Instance heap_bij_empty : Empty heap_bij := HeapBij ∅ _.
+Next Obligation. set_solver. Qed.
+
+Definition hb_shared_provs (bij : heap_bij) : gset prov :=
+  list_to_set (omap (λ x, if x.2 is HBShared p then Some p else None) (map_to_list (hb_bij bij))).
+
+Global Typeclasses Opaque hb_shared_provs.
+
+Lemma elem_of_hb_shared_provs bij p1:
+  p1 ∈ hb_shared_provs bij ↔ ∃ p2, hb_bij bij !! p2 = Some (HBShared p1).
+Proof.
+  rewrite /hb_shared_provs elem_of_list_to_set elem_of_list_omap.
+  setoid_rewrite elem_of_map_to_list'.
+  split.
+  - move => [[??] /= [??]]. case_match; simplify_eq/=. naive_solver.
+  - move => [??]. by eexists (_, _).
+Qed.
+
+Program Definition heap_bij_add_shared (p1 p2 : prov) (bij : heap_bij)
+        (H : p1 ∉ hb_shared_provs bij) :=
+  HeapBij (<[p2 := HBShared p1]> (hb_bij bij)) _.
+Next Obligation.
+  move => ??? Hnotin ????.
+  rewrite !lookup_insert_Some => ??. destruct_all?; simplify_eq/= => //. 3: by apply: hb_iff.
+  all: split => ?; simplify_eq; contradict Hnotin; apply elem_of_hb_shared_provs; naive_solver.
+Qed.
+
+Program Definition heap_bij_update_const (p : prov) (h : gmap loc val) (bij : heap_bij) :=
+  HeapBij (<[p := HBConstant (λ o, h !! (p, o))]> (hb_bij bij)) _.
+Next Obligation.
+  move => ???????.
+  rewrite !lookup_insert_Some => ??. destruct_all?; simplify_eq/= => //. by apply: hb_iff.
+Qed.
+
+Program Definition heap_bij_delete_prov (p : prov) (bij : heap_bij) :=
+  HeapBij (delete p (hb_bij bij)) _.
+Next Obligation.
+  move => ??????.
+  rewrite !lookup_delete_Some => ??. destruct_all?; simplify_eq/= => //. by apply: hb_iff.
+Qed.
+
+Lemma hb_shared_provs_add_shared p1 p2 bij H:
+  hb_shared_provs (heap_bij_add_shared p1 p2 bij H) ⊆ {[p1]} ∪ hb_shared_provs bij.
+Proof.
+  move => ?/elem_of_hb_shared_provs[/=?/lookup_insert_Some?].
+  set_unfold. rewrite elem_of_hb_shared_provs. naive_solver.
+Qed.
+
+Lemma hb_shared_provs_update_const p h bij:
+  hb_shared_provs (heap_bij_update_const p h bij) ⊆ hb_shared_provs bij.
+Proof.
+  move => ?. rewrite !elem_of_hb_shared_provs /=.
+  setoid_rewrite lookup_insert_Some. naive_solver.
+Qed.
+
+(* Global Instance heap_bij_subseteq : SubsetEq heap_bij := *)
+  (* λ bij1 bij2, ∀ p1 p2, hb_bij bij1 !! p2 = Some (HBShared p1) → hb_bij bij2 !! p2 = Some (HBShared p1). *)
+
+Definition heap_bij_auth (bij : heap_bij) : heap_bijUR :=
+  gmap_view_auth (DfracOwn 1) (hb_bij bij).
+
+Definition heap_bij_shared (p1 p2 : prov) : heap_bijUR :=
+  gmap_view_frag p2 DfracDiscarded (HBShared p1).
+
+Definition heap_bij_const (p : prov) (f : Z → option val) : heap_bijUR :=
+  gmap_view_frag p (DfracOwn 1) (HBConstant f).
+
+Lemma heap_bij_alloc_shared bij p1 p2 H:
+  p2 ∉ dom (gset _) (hb_bij bij) →
+  heap_bij_auth bij ~~> heap_bij_auth (heap_bij_add_shared p1 p2 bij H) ⋅ heap_bij_shared p1 p2.
+Proof. move => ?. apply gmap_view_alloc; [|done]. by apply not_elem_of_dom. Qed.
+
+Lemma heap_bij_shared_lookup p1 p2 bij :
+  ✓ (heap_bij_auth bij ⋅ heap_bij_shared p1 p2) →
+  hb_bij bij !! p2 = Some (HBShared p1).
+Proof. move => /gmap_view_both_valid_L. naive_solver. Qed.
+
+Lemma heap_bij_alloc_const bij p h:
+  p ∉ dom (gset _) (hb_bij bij) →
+  heap_bij_auth bij ~~> heap_bij_auth (heap_bij_update_const p h bij) ⋅ heap_bij_const p (λ o, h !! (p, o)).
+Proof. move => ?. apply gmap_view_alloc; [|done]. by apply not_elem_of_dom. Qed.
+
+Lemma heap_bij_const_lookup p f bij :
+  ✓ (heap_bij_auth bij ⋅ heap_bij_const p f) →
+  hb_bij bij !! p = Some (HBConstant f).
+Proof. move => /gmap_view_both_valid_L. naive_solver. Qed.
+
+Lemma heap_bij_frag_update_const bij p f h:
+  heap_bij_auth bij ⋅ heap_bij_const p f ~~>
+  heap_bij_auth (heap_bij_update_const p h bij) ⋅ heap_bij_const p (λ o, h !! (p, o)).
+Proof. apply gmap_view_update. Qed.
+
+(** ** val_in_bij *)
+Definition val_in_bij (r : heap_bijUR) (v1 v2 : val) : Prop :=
+  match v1, v2 with
+  | ValNum n1, ValNum n2 => n1 = n2
+  | ValBool b1, ValBool b2 => b1 = b2
+  | ValLoc l1, ValLoc l2 => heap_bij_shared l1.1 l2.1 ≼ r /\ l1.2 = l2.2
+  | _, _ => False
+  end.
+
+Lemma val_in_bij_mono r r' v1 v2:
+  val_in_bij r v1 v2 →
+  core r ≼ r' →
+  val_in_bij r' v1 v2.
+Proof.
+  destruct v1, v2 => //=. move => [??] ?. split; [|done].
+  rewrite -(core_id_core (heap_bij_shared _ _)).
+  etrans; [|done]. by apply cmra_core_mono.
+Qed.
+
+(** ** expr_in_bij *)
+Fixpoint expr_in_bij (r : heap_bijUR) (e1 e2 : expr) {struct e1} : Prop :=
+  match e1, e2 with
+  | Var v, Var v' => v = v'
+  | Val v, Val v' => val_in_bij r v v'
+  | BinOp e1 o e2, BinOp e1' o' e2' => o = o' ∧ expr_in_bij r e1 e1' ∧ expr_in_bij r e2 e2'
+  | Load e, Load e' => expr_in_bij r e e'
+  | Store e1 e2, Store e1' e2' => expr_in_bij r e1 e1' ∧ expr_in_bij r e2 e2'
+  | Alloc e, Alloc e' => expr_in_bij r e e'
+  | Free e, Free e' => expr_in_bij r e e'
+  | If e e1 e2, If e' e1' e2' => expr_in_bij r e e' ∧ expr_in_bij r e1 e1' ∧ expr_in_bij r e2 e2'
+  | LetE v e1 e2, LetE v' e1' e2' => v = v' ∧ expr_in_bij r e1 e1' ∧ expr_in_bij r e2 e2'
+  | Call f args, Call f' args' => f = f' ∧ length args = length args' ∧
+                                   Forall id (zip_with (expr_in_bij r) args args')
+  | UbE, UbE => True
+  | ReturnExt b e, ReturnExt b' e' => b = b' ∧ expr_in_bij r e e'
+  | Waiting b, Waiting b' => b = b'
+  | _, _ => False
+  end.
+
+Lemma Forall2_bij_val_inv_l r vl el :
+  Forall2 (expr_in_bij r) (Val <$> vl) el →
+  ∃ vl', el = Val <$> vl' ∧ Forall2 (val_in_bij r) vl vl'.
+Proof.
+  elim: vl el; csimpl. { move => ? /Forall2_nil_inv_l->. by eexists []. }
+  move => ?? IH ? /(Forall2_cons_inv_l _ _)[v' [?[?[/IH[?[??]]?]]]]; subst.
+  destruct v' => //. eexists (_::_). split; [done|]. by econs.
+Qed.
+
+Lemma Forall2_bij_val_inv_r r vl el :
+  Forall2 (expr_in_bij r) el (Val <$> vl) →
+  ∃ vl', el = Val <$> vl' ∧ Forall2 (val_in_bij r) vl' vl.
+Proof.
+  elim: vl el; csimpl. { move => ? /Forall2_nil_inv_r->. by eexists []. }
+  move => ?? IH ? /(Forall2_cons_inv_r _ _ _ _) [v' [?[?[/IH[?[??]] ?]]]]; subst.
+  destruct v' => //. eexists (_::_). split; [done|]. by econs.
+Qed.
+
+Lemma expr_in_bij_mono r r' e1 e2:
+  expr_in_bij r e1 e2 →
+  core r ≼ r' →
+  expr_in_bij r' e1 e2.
+Proof.
+  elim: e1 e2 => //=*; repeat case_match => //; try naive_solver (eauto using val_in_bij_mono).
+  destruct_all?; simplify_eq. split!.
+  revert select (Forall id _). generalize dependent args.
+  revert select (Forall _ _). elim. { by case. }
+  move => ????? []//=??? *; decompose_Forall_hyps. econs; naive_solver.
+Qed.
+
+Lemma expr_in_bij_subst r x v e v' e':
+  expr_in_bij r e e' →
+  val_in_bij r v v' →
+  expr_in_bij r (subst x v e) (subst x v' e').
+Proof.
+  elim: e e' => //= *; repeat (case_match => //); simplify_eq/=; repeat case_bool_decide => //; try naive_solver.
+  destruct_all?. rewrite !fmap_length. split!.
+  revert select (Forall _ _). generalize dependent args.
+  revert select (Forall _ _). elim. { by case. }
+  move => ????? []//=??? /(Forall_cons_1 _ _)[??]. econs; naive_solver.
+Qed.
+
+Lemma expr_in_bij_subst_l r xs vs e vs' e':
+  expr_in_bij r e e' →
+  Forall2 (val_in_bij r) vs vs' →
+  length xs = length vs →
+  expr_in_bij r (subst_l xs vs e) (subst_l xs vs' e').
+Proof.
+  move => He Hall. elim: Hall xs e e' He. { by case. }
+  move => ?????? IH []//=??????. apply: IH; [|lia]. by apply expr_in_bij_subst.
+Qed.
+
+Lemma expr_in_bij_static r e:
+  static_expr false e →
+  expr_in_bij r e e.
+Proof.
+  elim: e => //=; try naive_solver. { by case. }
+  move => ?? IH Hb. split!.
+  elim: IH Hb => //=; econs; naive_solver.
+Qed.
+
+(** ** ectx_in_bij *)
+Definition ectx_item_in_bij (r : heap_bijUR) (Ki Ki' : expr_ectx) : Prop :=
+  match Ki, Ki' with
+  | BinOpLCtx op e2, BinOpLCtx op' e2' => op = op' ∧ expr_in_bij r e2 e2'
+  | BinOpRCtx v1 op, BinOpRCtx v1' op' => op = op' ∧ val_in_bij r v1 v1'
+  | LoadCtx, LoadCtx => True
+  | StoreLCtx e2, StoreLCtx e2' => expr_in_bij r e2 e2'
+  | StoreRCtx v1, StoreRCtx v1' => val_in_bij r v1 v1'
+  | AllocCtx, AllocCtx => True
+  | FreeCtx, FreeCtx => True
+  | IfCtx e2 e3, IfCtx e2' e3' => expr_in_bij r e2 e2' ∧ expr_in_bij r e3 e3'
+  | LetECtx v e2, LetECtx v' e2' => v = v' ∧ expr_in_bij r e2 e2'
+  | CallCtx f vl el, CallCtx f' vl' el' => f = f' ∧ Forall2 (val_in_bij r) vl vl' ∧
+                                            Forall2 (expr_in_bij r) el el'
+  | ReturnExtCtx b, ReturnExtCtx b' => b = b'
+  | _, _ => False
+  end.
+
+Definition ectx_in_bij (r : heap_bijUR) (K1 K2 : list expr_ectx) : Prop :=
+  Forall2 (ectx_item_in_bij r) K1 K2.
+
+Lemma ectx_item_in_bij_mono r r' K1 K2:
+  ectx_item_in_bij r K1 K2 →
+  core r ≼ r' →
+  ectx_item_in_bij r' K1 K2.
+Proof.
+  destruct K1, K2 => //=; try naive_solver (eauto using expr_in_bij_mono, val_in_bij_mono).
+  move => [?[??]] ?. split_and!; [done|..].
+  all: apply: Forall2_impl; [done|]; eauto using expr_in_bij_mono, val_in_bij_mono.
+Qed.
+
+Lemma ectx_in_bij_mono r r' K1 K2:
+  ectx_in_bij r K1 K2 →
+  core r ≼ r' →
+  ectx_in_bij r' K1 K2.
+Proof. move => ??. apply: Forall2_impl; [done|]. move => *; by apply: ectx_item_in_bij_mono.  Qed.
+
+Lemma ectx_in_bij_cons r Ki K Ki' K':
+  ectx_in_bij r (Ki :: K) (Ki' :: K') ↔ ectx_item_in_bij r Ki Ki' ∧ ectx_in_bij r K K'.
+Proof. apply Forall2_cons. Qed.
+
+Lemma ectx_in_bij_app r Ki K Ki' K':
+  ectx_in_bij r Ki Ki' →
+  ectx_in_bij r K K' →
+  ectx_in_bij r (Ki ++ K) (Ki' ++ K').
+Proof. apply Forall2_app. Qed.
+
+Lemma ectx_in_bij_cons_inv_l r Ki K K':
+  ectx_in_bij r (Ki::K) K' →
+  ∃ Ki' K'', ectx_item_in_bij r Ki Ki' ∧ ectx_in_bij r K K'' ∧ K' = Ki' :: K''.
+Proof. apply Forall2_cons_inv_l. Qed.
+
+Lemma expr_in_bij_fill_item_2 r K1 K2 e1 e2 :
+  ectx_item_in_bij r K1 K2 →
+  expr_in_bij r e1 e2 →
+  expr_in_bij r (expr_fill_item K1 e1) (expr_fill_item K2 e2).
+Proof.
+  move => ??.
+  destruct K1, K2 => //; simplify_eq/=; destruct_all? => //.
+  rewrite !app_length /=. split_and!; [done|solve_length|].
+  apply Forall_zip_with_2. apply Forall2_app; [by apply Forall2_fmap|by econs].
+Qed.
+
+Lemma expr_in_bij_fill_2 r K1 K2 e1 e2 :
+  ectx_in_bij r K1 K2 →
+  expr_in_bij r e1 e2 →
+  expr_in_bij r (expr_fill K1 e1) (expr_fill K2 e2).
+Proof.
+  elim: K1 K2 e1 e2. { move => ??? /Forall2_nil_inv_l->. done. }
+  move => Ki1 K1 IH ??? /(Forall2_cons_inv_l _ _)[Ki2 [K2 [?[??]]]] ?; subst => /=.
+  apply: IH; [done|]. by apply expr_in_bij_fill_item_2.
+Qed.
+
+Lemma expr_in_bij_fill_item_l r Ki e1 e2 :
+  expr_in_bij r (expr_fill_item Ki e1) e2 →
+  ∃ Ki' e', e2 = expr_fill_item Ki' e' ∧ ectx_item_in_bij r Ki Ki' ∧ expr_in_bij r e1 e'.
+Proof.
+  destruct Ki, e2 => //= *; destruct_all?; simplify_eq; try case_match => //; simplify_eq. 10: {
+    revert select (Forall _ _) => /Forall_zip_with_1 Hall.
+    move: (Hall ltac:(done)) => /Forall2_app_inv_l[?[?[Hv[/(Forall2_cons_inv_l _ _)[?[?[?[??]]]]?]]]]. simplify_eq.
+    move: Hv => /Forall2_bij_val_inv_l[?[??]]. simplify_eq.
+    by eexists (CallCtx _ _ _), _.
+  }
+  all: (unshelve eexists _); [econs; shelve| naive_solver].
+Qed.
+
+Lemma expr_in_bij_fill_l r K e1 e2 :
+  expr_in_bij r (expr_fill K e1) e2 →
+  ∃ K' e', e2 = expr_fill K' e' ∧ ectx_in_bij r K K' ∧ expr_in_bij r e1 e'.
+Proof.
+  elim: K e1 e2 => /=. { move => *. eexists [], _. split!. econs. }
+  move => Ki K IH e1 e2 /IH[K'[?[?[?/expr_in_bij_fill_item_l?]]]].
+  destruct_all?; simplify_eq. eexists (_ :: _), _ => /=. split_and!; [done| |done].
+  by econs.
+Qed.
+
+Lemma eval_binop_bij o v1 v2 v1' v2' v r:
+  eval_binop o v1 v2 = Some v →
+  val_in_bij r v1' v1 →
+  val_in_bij r v2' v2 →
+  ∃ v', eval_binop o v1' v2' = Some v' ∧
+       val_in_bij r v' v.
+Proof.
+  destruct o, v1, v2, v1', v2' => //= *; destruct_all?; simplify_eq. all: split!.
+  lia.
+Qed.
+
+(** *** heap_in_bij *)
+Definition heap_in_bij (bij : heap_bij) (r : heap_bijUR) (h h' : heap_state) : Prop :=
+  ∀ p1 p2 o,
+  hb_bij bij !! p2 = Some (HBShared p1) →
+
+  (is_Some (h.(h_heap) !! (p1, o)) ↔ is_Some (h'.(h_heap) !! (p2, o)))
+  /\
+  ∀ v1 v2,
+  h.(h_heap)  !! (p1, o) = Some v1 →
+  h'.(h_heap) !! (p2, o) = Some v2 →
+  val_in_bij r v1 v2.
+
+Lemma heap_in_bij_mono bij r r' h h':
+  heap_in_bij bij r h h' →
+  core r ≼ r' →
+  heap_in_bij bij r' h h'.
+Proof.
+  move => Hbij ? ????. split; [by apply Hbij|].
+  move => ????. apply: val_in_bij_mono; [|done].
+  by eapply Hbij.
+Qed.
+
+Lemma heap_in_bij_mono_bij bij bij' r h h':
+  heap_in_bij bij r h h' →
+  (∀ p1 p2, hb_bij bij' !! p2 = Some (HBShared p1) → hb_bij bij !! p2 = Some (HBShared p1)) →
+  heap_in_bij bij' r h h'.
+Proof. unfold heap_in_bij => Hp ?????. apply: Hp. naive_solver. Qed.
+
+Lemma heap_in_bij_alive bij r h1 h2 l1 l2:
+  heap_in_bij bij r h1 h2 →
+  heap_alive h2 l2 →
+  hb_bij bij !! l2.1 = Some (HBShared l1.1) →
+  l1.2 = l2.2 →
+  heap_alive h1 l1.
+Proof.
+  move => ? Hbij ??. destruct l1 as [p1 ?], l2 as [p2 o]; simplify_eq/=.
+  unfold heap_in_bij, heap_alive in *. naive_solver.
+Qed.
+
+Lemma heap_in_bij_lookup bij r h1 h2 l1 l2 v:
+  h_heap h2 !! l2 = Some v →
+  heap_in_bij bij r h1 h2 →
+  hb_bij bij !! l2.1 = Some (HBShared l1.1) →
+  l1.2 = l2.2 →
+  ∃ v', h_heap h1 !! l1 = Some v' ∧ val_in_bij r v' v.
+Proof.
+  move => ? Hbij ??. destruct l1 as [p1 ?], l2 as [p2 o]; simplify_eq/=.
+  have [[? H2]?]:= Hbij _ _ o ltac:(done).
+  have [??]:= H2 ltac:(done).
+  naive_solver.
+Qed.
+
+Lemma heap_in_bij_update bij r h1 h2 l1 l2 v1 v2:
+  heap_in_bij bij r h1 h2 →
+  val_in_bij r v1 v2 →
+  hb_bij bij !! l2.1 = Some (HBShared l1.1) →
+  l1.2 = l2.2 →
+  heap_in_bij bij r (heap_update h1 l1 v1) (heap_update h2 l2 v2).
+Proof.
+  move => Hbij ???. destruct l1 as [p1 ?], l2 as [p2 o]; simplify_eq/=.
+  move => p1' p2' o' /=?. have : p1 = p1' ↔ p2 = p2' by apply: hb_iff.
+  split.
+  - rewrite !lookup_alter_is_Some. by apply Hbij.
+  - move => ?? /lookup_alter_Some[[?[?[??]]]|[??]] /lookup_alter_Some[[?[?[??]]]|[??]]; simplify_eq.
+    all: try by eapply Hbij. all: naive_solver.
+Qed.
+
+Lemma heap_in_bij_update_r bij r h1 h2 l2 v2:
+  heap_in_bij bij r h1 h2 →
+  (∀ p, hb_bij bij !! l2.1 = Some (HBShared p) → False) →
+  heap_in_bij bij r h1 (heap_update h2 l2 v2).
+Proof.
+  move => Hbij Hin ? ??? /=.
+  rewrite !lookup_alter_ne. 1: by apply Hbij.
+  naive_solver.
+Qed.
+
+Lemma heap_in_bij_alloc l1 l2 hi hs n bij r H:
+  heap_in_bij bij r hi hs →
+  heap_is_fresh hi l1 →
+  heap_is_fresh hs l2 →
+  heap_in_bij (heap_bij_add_shared l1.1 l2.1 bij H) r (heap_alloc hi l1 n) (heap_alloc hs l2 n).
+Proof.
+  move => /= Hbij [Hi1 ?] [Hi2 ?]  p1 p2 o /= /lookup_insert_Some[[??]|[??]]; simplify_eq.
+  - destruct l1 as [p1 ?], l2 as [p2 ?]; simplify_eq/=.
+    rewrite !lookup_union_l'.
+    2: { apply eq_None_ne_Some => ??. apply Hi2. by apply: (heap_wf _ (_, _)). }
+    2: { apply eq_None_ne_Some => ??. apply Hi1. by apply: (heap_wf _ (_, _)). }
+    split.
+    + rewrite !list_to_map_lookup_is_Some. f_equiv => ?. rewrite !elem_of_list_fmap.
+      f_equiv => ?. naive_solver.
+    + move => ?? /(elem_of_list_to_map_2 _ _ _)/elem_of_list_fmap[?[??]].
+      move => /(elem_of_list_to_map_2 _ _ _)/elem_of_list_fmap[?[??]]. by simplify_eq/=.
+  -
+    have ? : p1 ≠ l1.1. { contradict H. apply elem_of_hb_shared_provs. naive_solver. }
+    (* have ? : p2 ≠ l2.1 by contradict H2; set_unfold; left; left; eexists (_, _); naive_solver. *)
+    have [Hbij1 Hbij2]:= Hbij p1 p2 o ltac:(set_solver).
+    rewrite !lookup_union_r.
+    2, 3: apply not_elem_of_list_to_map_1;
+        move => /elem_of_list_fmap[[[??]?] [?/elem_of_list_fmap[?[??]]]]; simplify_eq/=.
+    split; [done|] => *. apply: val_in_bij_mono; [naive_solver|]. apply cmra_included_core.
+Qed.
+
+Lemma heap_in_bij_alloc_r l2 hi hs n bij r:
+  heap_in_bij bij r hi hs →
+  (∀ p, hb_bij bij !! l2.1 = Some (HBShared p) → False) →
+  heap_in_bij bij r hi (heap_alloc hs l2 n).
+Proof.
+  move => /= Hbij Hin ???? /=. rewrite lookup_union_r. 1: by apply Hbij.
+  apply not_elem_of_list_to_map_1.
+  move => /elem_of_list_fmap[[??][?/elem_of_list_fmap[?[??]]]]; simplify_eq/=.
+  naive_solver.
+Qed.
+
+Lemma heap_in_bij_free r hi hs l1 l2 bij:
+  heap_in_bij bij r hi hs →
+  hb_bij bij !! l2.1 = Some (HBShared l1.1) →
+  heap_in_bij bij r (heap_free hi l1) (heap_free hs l2).
+Proof.
+  move => Hbij Hin p1 p2 o /=?.
+  have [Hbij1 Hbij2]:= Hbij p1 p2 o ltac:(done).
+  have ?: p1 = l1.1 ↔ p2 = l2.1 by apply: hb_iff.
+  split.
+  - rewrite !map_filter_lookup /=. destruct (h_heap hi !! (p1, o)), (h_heap hs !! (p2, o)) => //=.
+    all: repeat case_option_guard => //; naive_solver.
+  - move => ??. rewrite !map_filter_lookup => /bind_Some[?[??]] /bind_Some[?[??]].
+    repeat case_option_guard => //; naive_solver.
+Qed.
+
+Lemma heap_in_bij_free_r l2 hi hs bij r:
+  heap_in_bij bij r hi hs →
+  (∀ p, hb_bij bij !! l2.1 = Some (HBShared p) → False) →
+  heap_in_bij bij r hi (heap_free hs l2).
+Proof.
+  move => /= Hbij Hin ???? /=. rewrite map_filter_lookup_true. 1: by apply Hbij.
+  naive_solver.
+Qed.
+
+(** *** heap_preserved *)
+Definition heap_preserved (bij : heap_bij) (h : heap_state) :=
+  ∀ l f, hb_bij bij !! l.1 = Some (HBConstant f) → h.(h_heap) !! l = f l.2.
+
+Lemma heap_preserved_mono bij1 bij2 h:
+  heap_preserved bij1 h →
+  (∀ p f, hb_bij bij2 !! p = Some (HBConstant f) → hb_bij bij1 !! p = Some (HBConstant f)) →
+  heap_preserved bij2 h.
+Proof. unfold heap_preserved => Hp ????. apply: Hp. naive_solver. Qed.
+
+Lemma heap_preserved_lookup_r bij h f l v:
+  h_heap h !! l = v →
+  heap_preserved bij h →
+  hb_bij bij !! l.1 = Some (HBConstant f) →
+  f l.2 = v.
+Proof. move => Hl Hp ?. by rewrite -Hp. Qed.
+
+Lemma heap_preserved_update l v h bij:
+  heap_preserved bij h →
+  (∀ f, hb_bij bij !! l.1 = Some (HBConstant f) → False) →
+  heap_preserved bij (heap_update h l v).
+Proof.
+  move => Hp ???? /=. rewrite lookup_alter_ne; [by eapply Hp|naive_solver].
+Qed.
+
+Lemma heap_preserved_alloc l n h bij:
+  heap_preserved bij h →
+  (∀ f, hb_bij bij !! l.1 = Some (HBConstant f) → False) →
+  heap_preserved bij (heap_alloc h l n).
+Proof.
+  move => Hp ? l' f /= ?. rewrite lookup_union_r; [by apply Hp|].
+  apply not_elem_of_list_to_map_1 => /elem_of_list_fmap[[[??]?] [?/elem_of_list_fmap[?[??]]]]; simplify_eq/=.
+  naive_solver.
+Qed.
+
+Lemma heap_preserved_free l h bij:
+  heap_preserved bij h →
+  (∀ f, hb_bij bij !! l.1 = Some (HBConstant f) → False) →
+  heap_preserved bij (heap_free h l).
+Proof.
+  move => Hp ? l' f ? /=. rewrite map_filter_lookup. etrans; [|by eapply Hp].
+  destruct (h_heap h !! l') => //=. case_option_guard => //. destruct l, l'; naive_solver.
+Qed.
+
+Lemma heap_preserved_add_shared p1 p2 bij H h:
+  heap_preserved bij h →
+  heap_preserved (heap_bij_add_shared p1 p2 bij H) h.
+Proof. move => Hp l f /= /lookup_insert_Some[[??//]|[??]]. by apply Hp. Qed.
+
+Lemma heap_preserved_update_const p bij h:
+  heap_preserved (heap_bij_delete_prov p bij) h →
+  heap_preserved (heap_bij_update_const p (h_heap h) bij) h.
+Proof.
+  move => Hp l f /= /lookup_insert_Some[[??]|[??]]; simplify_eq. 1: by destruct l.
+  apply: Hp => /=. rewrite lookup_delete_Some. done.
+Qed.
+
+Definition imp_heap_bij_pre (e : imp_event) (s : heap_bijUR) : prepost (imp_event * heap_bijUR) :=
+  let ho := heap_of_event e.2 in
+  pp_quant $ λ bij,
+  pp_quant $ λ vsi,
+  pp_quant $ λ hi,
+  pp_quant $ λ r',
+  pp_own (heap_bij_auth bij ⋅ r') s $ λ y,
+  (* TODO: should we also have the following for hi? We don't need it so far... *)
+  pp_prop (hb_shared_provs bij ⊆ h_provs ho) $
+  pp_prop (Forall2 (val_in_bij r') (vals_of_event e.2) vsi) $
+  pp_prop (heap_in_bij bij r' ho hi) $
+  pp_prop (heap_preserved bij hi) $
+  pp_end ((e.1, event_set_vals_heap e.2 vsi hi), y).
+
+Definition imp_heap_bij_post (e : imp_event) (s : heap_bijUR) : prepost (imp_event * heap_bijUR) :=
+  let hi := heap_of_event e.2 in
+  pp_quant $ λ bij,
+  pp_quant $ λ vso,
+  pp_quant $ λ ho,
+  pp_quant $ λ r',
+  pp_update (heap_bij_auth bij ⋅ r') s $ λ y,
+  (* TODO: should we also have the following for hi? We don't need it so far... *)
+  pp_prop (hb_shared_provs bij ⊆ h_provs ho) $
+  pp_prop (Forall2 (val_in_bij r') vso (vals_of_event e.2)) $
+  pp_prop (heap_in_bij bij r' ho hi) $
+  pp_prop (heap_preserved bij hi) $
+  pp_end ((e.1, event_set_vals_heap e.2 vso ho), y).
+
+Definition imp_heap_bij (m : module imp_event) : module imp_event :=
+  mod_prepost imp_heap_bij_pre imp_heap_bij_post m.
+
+Definition initial_imp_heap_bij_state (m : module imp_event) (σ : m.(m_state)) :=
+  (@SMFilter imp_event, σ, (@PPOutside imp_event imp_event, @ε heap_bijUR _)).
+
+Local Ltac split_solve :=
+  match goal with
+  | |- heap_in_bij ?p _ _ _ => is_evar p; eassumption
+  | |- event_set_vals_heap _ _ _ = event_set_vals_heap _ _ _ => reflexivity
+(*   | |- ?a ⊆ ?b => *)
+(*       assert_fails (has_evar a); assert_fails (has_evar b); etrans; [eassumption|] *)
+(*   | |- ?a ⊆ ?b => *)
+(*       assert_fails (has_evar a); assert_fails (has_evar b); etrans; [|eassumption] *)
+(*   | |- heap_preserved ?p ?a ?b => *)
+(*       assert_fails (has_evar p); assert_fails (has_evar a); assert_fails (has_evar b); etrans; [eassumption|] *)
+  end.
+Local Ltac split_tac ::=
+  repeat (original_split_tac; try split_solve).
+
+Lemma imp_heap_bij_combine fns1 fns2 m1 m2 σ1 σ2 `{!VisNoAll m1} `{!VisNoAll m2}:
+  trefines (MS (imp_prod fns1 fns2 (imp_heap_bij m1) (imp_heap_bij m2))
+               (MLFNone, [], initial_imp_heap_bij_state m1 σ1,
+                 initial_imp_heap_bij_state m2 σ2))
+           (MS (imp_heap_bij (imp_prod fns1 fns2 m1 m2))
+               (initial_imp_heap_bij_state (imp_prod _ _ _ _)
+                  (MLFNone, [], σ1, σ2) )
+).
+Proof.
+  unshelve apply: mod_prepost_link. { exact
+      (λ ips r1 r2 r ics1 ics2,
+          ics1 = ics2 ∧
+            ✓ r ∧
+       ((ips = SPNone ∧
+          r ≡ r1 ⋅ r2) ∨
+        ((ips = SPLeft ∧
+          r ~~> r1 ⋅ r2) ∨
+         (ips = SPRight ∧
+          r ~~> r1 ⋅ r2)))). }
+  { move => ?? [] /=*; naive_solver. }
+  { split!. 1: apply ucmra_unit_valid. 1: by rewrite left_id.  }
+  all: move => r1 r2 r ics1 ics2.
+  - move => e ics' e' /= ? [? [Hvalid [[? Hequiv]|[?|?]]]] *; destruct_all?; simplify_eq/=.
+    split!.
+    { apply: cmra_valid_included; [done|]. apply cmra_mono_l.
+      rewrite Hequiv. by apply cmra_included_l. }
+    all: split!.
+    1: by destruct e.
+    1: by rewrite Hequiv assoc.
+  - move => e ics' e' /= ? [? [Hvalid [[? Hequiv]|[?|?]]]] *; destruct_all?; simplify_eq/=.
+    split!.
+    { apply: cmra_valid_included; [done|]. apply cmra_mono_l.
+      rewrite Hequiv. by apply cmra_included_r. }
+    all: split!.
+    1: by destruct e.
+    1: by rewrite (comm _ r1) -(assoc _ _ r2) (comm _ r2) Hequiv.
+  - move => [? e] /= [? [Hvalid [?|[[? Hr]|?]]]] *; destruct_all?; simplify_eq/=.
+    revert select (_ ~~> _) => Hupdate. rewrite Hupdate in Hr.
+    split!.
+    1: { apply: cmra_valid_included; [by apply: ucmra_discrete_update_valid|].
+         apply cmra_mono_r. by apply cmra_included_l. }
+    all: rewrite ?heap_of_event_event_set_vals_heap; split!.
+    1: { rewrite vals_of_event_event_set_vals_heap //. by apply: Forall2_length. }
+    1: done.
+    all: split!.
+    1: { rewrite comm -assoc (comm _ r2) assoc. done. }
+    1: by destruct e.
+    1: by destruct e.
+  - move => [? e] /= [? [Hvalid [?|[[? Hr]|?]]]] *; destruct_all?; simplify_eq/=.
+    revert select (_ ~~> _) => Hupdate. rewrite Hupdate in Hr.
+    split!.
+    1: by destruct e.
+    3: done.
+    1: { rewrite assoc. done. }
+    1: { apply: cmra_valid_included; [by apply: ucmra_discrete_update_valid|].
+         apply cmra_mono_r. by apply cmra_included_r. }
+  - move => [? e] /= [? [Hvalid [?|[?|[? Hr]]]]] *; destruct_all?; simplify_eq/=.
+    revert select (_ ~~> _) => Hupdate. rewrite Hupdate in Hr.
+    split!.
+    1: { apply: cmra_valid_included; [by apply: ucmra_discrete_update_valid|].
+         rewrite comm. apply cmra_mono_l. by apply cmra_included_l. }
+    all: rewrite ?heap_of_event_event_set_vals_heap; split!.
+    1: { rewrite vals_of_event_event_set_vals_heap //. by apply: Forall2_length. }
+    1: done.
+    all: split!.
+    1: { rewrite -assoc (comm _ r1) assoc comm. done. }
+    1: by destruct e.
+    1: by destruct e.
+  - move => [? e] /= [? [Hvalid [?|[?|[? Hr]]]]] *; destruct_all?; simplify_eq/=.
+    revert select (_ ~~> _) => Hupdate. rewrite Hupdate in Hr.
+    split!.
+    1: by destruct e.
+    3: done.
+    1: { rewrite (comm _ r1) assoc comm. done. }
+    1: { apply: cmra_valid_included. 1: by apply: ucmra_discrete_update_valid.
+         apply cmra_mono_l. by apply cmra_included_r. }
+Qed.
+
+Local Ltac split_solve ::=
+  match goal with
+  | |- expr_fill (?K' ++ ?K) _ = expr_fill ?K _ =>
+      assert_fails (has_evar K'); assert_fails (has_evar K); apply expr_fill_app
+  | |- expr_fill ?K _ = expr_fill ?K _ =>
+      assert_fails (has_evar K); reflexivity
+  | |- Is_true (static_expr _ (expr_fill _ _)) => apply static_expr_expr_fill
+  | |- expr_in_bij ?b (expr_fill _ _) (expr_fill _ _) =>
+      assert_fails (has_evar b); apply expr_in_bij_fill_2
+  | |- ectx_in_bij ?b (_ ++ _) (_ ++ _) => assert_fails (has_evar b); by apply ectx_in_bij_app
+  end.
+Local Ltac split_tac ::=
+  repeat (original_split_tac; try split_solve).
+
+Lemma imp_heap_bij_imp_refl fns:
+  trefines (MS imp_module (initial_imp_state fns))
+           (MS (imp_heap_bij imp_module)
+               (initial_imp_heap_bij_state imp_module (initial_imp_state fns))).
+Proof.
+  pose (R := λ (b : bool) (r1 r2 : heap_bijUR), r1 ≼ r2).
+  apply: (imp_prepost_proof R); unfold R in *.
+  { move => ? ?. naive_solver. }
+  move => n K1 K2 f fn1 vs1 h1 r0 ?? /= bij *.
+  split!. move => ?. split; [solve_length|].
+  move => Hcall Hret.
+  unshelve apply: tsim_remember. { simpl. exact (λ _ '(Imp ei hi fnsi) '(ips, Imp es hs fnss, (pp, r')),
+    ∃ bij' ei' es' rvs,
+    fnsi = fns ∧ fnss = fns ∧
+    r' ~~> heap_bij_auth bij' ⋅ core rvs ⋅ r0 ∧
+    ✓ r' ∧
+    heap_preserved bij' hs ∧
+    ei = expr_fill K1 ei' ∧
+    es = expr_fill K2 es' ∧
+    expr_in_bij (core rvs) ei' es' ∧
+    heap_in_bij bij' (core rvs) hi hs ∧
+    hb_shared_provs bij' ⊆ h_provs hi ∧
+    pp = PPInside ∧
+    static_expr true ei' ∧
+    ips = SMProg
+ ). }
+  { split!.
+    { apply cmra_update_op; [|done]. apply cmra_update_op; [done|]. apply cmra_update_included.
+      apply cmra_included_core. }
+    all: split!.
+    { apply expr_in_bij_subst_l; [| |solve_length].
+      - apply expr_in_bij_static. apply fd_static.
+      - apply: Forall2_impl; [done|]. move => ???. by apply: val_in_bij_mono. }
+    { by apply: heap_in_bij_mono. }
+    { apply static_expr_subst_l; [|solve_length]. apply static_expr_mono. apply fd_static. }  }
+  { naive_solver. }
+  move => /= n' ? Hloop [ei hi fnsi] [[ips [es hs fnss]] [pp r]] ?. destruct_all?; simplify_eq.
+  destruct (to_val ei') eqn:?.
+  - destruct ei' => //; simplify_eq/=. destruct es' => //; simplify_eq/=.
+    apply Hret; [done|]. clear Hloop Hret Hcall. split!.
+    1: done. all: split!.
+    1: { by econs; [|done]. }
+    1: done.
+  - (* TODO: remove this use of EM *)
+    have [?|?]:= EM (∃ K f vs, fns !! f = None ∧ ei' = expr_fill K (Call f (Val <$> vs))).
+    + destruct_all?; simplify_eq/=.
+      revert select (expr_in_bij _ (expr_fill _ _) _) => /expr_in_bij_fill_l[?[?[?[??]]]].
+      destruct_all?; simplify_eq/=.
+      revert select (Is_true (static_expr _ _)) => /static_expr_expr_fill/=[??]//.
+      case_match => //; destruct_all?; simplify_eq/=.
+      revert select (Forall id _) => /Forall_zip_with_1 Hall.
+      move: (Hall ltac:(done)) => /Forall2_bij_val_inv_l[?[??]]; simplify_eq.
+      apply: Hcall; [done..| | |].
+      1,2: by apply Forall2_fmap_l, Forall_Forall2_diag, Forall_true.
+      clear Hret. split!.
+      1: { etrans; [done|]. rewrite cmra_core_dup assoc -assoc. done. }
+      all: split!.
+      1: { by apply cmra_included_r. }
+      move => *. decompose_Forall_hyps. split!.
+      apply Hloop; [done|]. split!.
+      1: { rewrite -!assoc. apply cmra_update_op; [done|].
+           etrans. { apply cmra_update_op; [done|]. by apply cmra_update_included. }
+           rewrite assoc. apply cmra_update_op; [|done].
+           apply cmra_update_included. apply cmra_included_core. }
+      all: split!.
+      { apply: ectx_in_bij_mono; [done|]. apply cmra_core_mono. by apply cmra_included_r. }
+      { apply: val_in_bij_mono; [done|]. apply cmra_core_mono. by apply cmra_included_l. }
+      { apply: heap_in_bij_mono; [done|]. apply cmra_core_mono. by apply cmra_included_l. }
+    + tstep_both.
+      apply steps_impl_step_end => ?? /= Hprim.
+      move: Hprim => /prim_step_inv[//|??].
+      destruct_all?; simplify_eq.
+      revert select (expr_in_bij _ (expr_fill _ _) _) => /expr_in_bij_fill_l[?[?[?[??]]]].
+      destruct_all?; simplify_eq.
+      revert select (Is_true (static_expr _ _)) => /static_expr_expr_fill/=[??]//.
+      invert_all' @head_step; destruct_all?; simplify_eq/=.
+      all: repeat (case_match; destruct_all? => //); simplify_eq.
+      * tstep_s => ? /eval_binop_bij Hbin. have [?[??]]:= Hbin _ _ _ ltac:(done) ltac:(done).
+        tend. split!. apply: Hloop; [done|]. split!. 1: done. all: split!.
+      * tstep_s => *; simplify_eq/=.
+        destruct v1 => //; simplify_eq/=; destruct_all?; simplify_eq/=. tend.
+        efeed pose proof heap_in_bij_lookup as Hl; [done|done| |done|destruct_all?].
+        { apply heap_bij_shared_lookup.
+          apply: cmra_valid_included; [by apply: ucmra_discrete_update_valid|].
+          apply: cmra_included_op_l. by apply: cmra_mono_l. }
+        split!. 1: done.
+        apply: Hloop; [done|]. split!. 1: done. all: split!.
+      * tstep_s => l' *; simplify_eq/=.
+        destruct v1 => //; simplify_eq/=; destruct_all?; simplify_eq/=. tend.
+        have ? : hb_bij bij' !! l'.1 = Some (HBShared l.1). {
+          apply heap_bij_shared_lookup.
+          apply: cmra_valid_included; [by apply: ucmra_discrete_update_valid|].
+          apply: cmra_included_op_l. by apply: cmra_mono_l.
+        }
+        split!.
+        1: { by apply: heap_in_bij_alive. }
+        apply: Hloop; [done|]. split!. 1: done. all: split!.
+        1: apply heap_preserved_update; [done|naive_solver].
+        1: by apply heap_in_bij_update.
+      * tstep_s => *; simplify_eq/=.
+        set (l' := (heap_fresh (dom _ (hb_bij bij')) hs)).
+        eexists l'. split; [apply heap_fresh_is_fresh|] => *; simplify_eq/=. tend.
+        destruct v => //; simplify_eq/=; destruct_all?; simplify_eq/=.
+        split!.
+        apply Hloop; [done|].
+        unshelve eexists (heap_bij_add_shared l.1 l'.1 bij' _).
+        { abstract (apply: not_elem_of_weaken; [|done]; unfold heap_is_fresh in *; naive_solver). }
+        split!.
+        1: { etrans; [done|]. apply cmra_update_op; [|done].
+             rewrite heap_bij_alloc_shared; [|apply (heap_fresh_not_in (dom _ (hb_bij bij')) hs)].
+             rewrite -assoc. apply cmra_update_op; [done|].
+             apply cmra_update_included, cmra_included_core. }
+        all: split!.
+        1: { apply heap_preserved_alloc; [|by move => *; simplify_map_eq].
+             by apply heap_preserved_add_shared. }
+        1: { apply: ectx_in_bij_mono; [done| ]. apply cmra_core_mono. apply cmra_included_r. }
+        1: { rewrite - {1}(core_id_core (heap_bij_shared _ _)). apply cmra_core_mono. apply cmra_included_l. }
+        1: unfold heap_is_fresh in *; naive_solver.
+        1: { apply: (heap_in_bij_alloc l l'); [|done|apply heap_fresh_is_fresh].
+             apply: heap_in_bij_mono; [done|]. apply cmra_core_mono. apply cmra_included_r. }
+        1: { etrans; [apply hb_shared_provs_add_shared|]. set_solver. }
+      * tstep_s => l' *; simplify_eq/=. tend.
+        destruct v => //; simplify_eq/=; destruct_all?; simplify_eq/=.
+        have ? : hb_bij bij' !! l'.1 = Some (HBShared l.1). {
+          apply heap_bij_shared_lookup.
+          apply: cmra_valid_included; [by apply: ucmra_discrete_update_valid|].
+          apply: cmra_included_op_l. by apply: cmra_mono_l.
+        }
+        split!. 1: by apply: heap_in_bij_alive. apply: Hloop; [done|].
+        split!. 1: done. all: split!.
+        1: apply heap_preserved_free; [done|naive_solver].
+        1: by apply heap_in_bij_free.
+      * tstep_s => *; simplify_eq/=. destruct v => //; simplify_eq/=. tend.
+        split!. apply: Hloop; [done|]. split!. 1: done. all: split!. all: by case_match.
+      * tstep_s. tend. split!. apply: Hloop; [done|]. split!. 1: done. all: split!.
+        1: by apply expr_in_bij_subst.
+        1: by apply static_expr_subst.
+      * by tstep_s.
+      * revert select (Forall id _) => /Forall_zip_with_1 Hall.
+        move: (Hall ltac:(done)) => /Forall2_bij_val_inv_l[?[??]]; simplify_eq.
+        tstep_s. left. split! => ?. tend. split!; [solve_length|].
+        apply Hloop; [done|]. split!. 1: done. all: split!.
+        1: { apply expr_in_bij_subst_l; [|done|solve_length]. apply expr_in_bij_static. apply fd_static. }
+        apply static_expr_subst_l; [|solve_length]. apply static_expr_mono. apply fd_static.
+      * naive_solver.
+Qed.
+
+Lemma imp_heap_bij_imp_closed m σ:
+  trefines (MS (imp_closed (imp_heap_bij m)) (SMFilter, initial_imp_heap_bij_state m σ, ICStart))
+           (MS (imp_closed m) (SMFilter, σ, ICStart)).
+Proof.
+  apply tsim_implies_trefines => /= n.
+  unshelve apply: tsim_remember. { simpl. exact (λ _
+          '(σm1, (σf, σ1, (pp, r)), σc1)
+          '(σm2, σ2, σc2),
+           σ1 = σ2 ∧ σc1 = σc2 ∧ ✓ r ∧
+             ((σc1 = ICStart ∧ σf = SMFilter ∧ pp = PPOutside ∧ σm1 = σm2 ∧ σm2 = SMFilter ∧ r = ε) ∨
+              ( ((∃ e, σf = SMProgRecv e ∧ σm2 = SMProgRecv e) ∨ (σf = SMProg ∧ σm2 = SMProg)
+                 ) ∧ σm1 = SMProg ∧ σc1 = ICRunning ∧ pp = PPInside))
+                             ). }
+  { split!. apply ucmra_unit_valid. } { done. }
+  move => {}n _ /= Hloop [[σm1 [[σf σ1] [pp r]]] σc1] [[σm2 σ2] σc2] ?. destruct_all?; simplify_eq/=.
+  - tstep_i. apply steps_impl_step_end => ???. invert_all' @m_step; simplify_eq/=. split!.
+    tstep_s. eexists (Some (inr _)). split!. apply: steps_spec_step_end; [econs|] => ??. simplify_eq/=.
+    tstep_i. apply steps_impl_step_end => ???. invert_all @m_step. split!.
+    tstep_s. eexists (Some (inl _)). split!. apply: steps_spec_step_end; [econs|] => ??. simplify_eq/=.
+    tstep_i => ??; simplify_eq/=.
+    tstep_i. eexists ∅, (ValNum <$> vs), initial_heap_state, ε. split!.
+    1: { rewrite !right_id. by apply gmap_view_auth_dfrac_valid. }
+    1: { apply Forall2_fmap. apply Forall_Forall2_diag. by apply Forall_true. }
+    apply: Hloop; [done|]. split!.
+    1: { rewrite !right_id. by apply gmap_view_auth_dfrac_valid. }
+  - tstep_both. apply steps_impl_step_end => κ ??. case_match => *; simplify_eq.
+    + tstep_s.  eexists (Some _). split; [done|]. apply: steps_spec_step_end; [done|] => ??. tend. split!; [done|].
+      apply: Hloop; [done|]. split!.
+    + tstep_s. eexists None. apply: steps_spec_step_end; [done|] => ??. tend. split!; [done|].
+      apply: Hloop; [done|]. split!.
+  - tstep_both. apply steps_impl_step_end => κ ??. tstep_s. eexists _. apply: steps_spec_step_end; [done|] => ??.
+    case_match; tend; (split!; [done|]). 2: { apply: Hloop; [done|]. split!. }
+    tstep_i => ? vs *. tstep_both => *.
+    apply steps_impl_step_end => ???. invert_all @m_step => ?; simplify_eq.
+    + destruct i as [? [? vs' |]]; simplify_eq/=.
+      tstep_s. eexists (Some _). split!.
+      apply: steps_spec_step_end; [econs|]=> /=??. destruct_all?; simplify_eq/=. tend.
+      split!.
+      tstep_both. apply steps_impl_step_end => ???. invert_all @m_step.
+      tstep_s. eexists (None). apply: steps_spec_step_end; [econs|]=> /=??. destruct_all?; simplify_eq/=. tend.
+      have ?: vs0 = ValNum <$> vs'0. {
+        revert select (m_step _ _ _ _) => _.
+        revert select (Forall2 _ _ _). elim: vs'0 vs0; csimpl => *; decompose_Forall_hyps => //.
+        match goal with |- ?x :: _ = _ => destruct x; simplify_eq/= => // end. naive_solver.
+      } subst.
+      split!; [done|].
+      tstep_i. apply steps_impl_step_end => ???. invert_all @m_step. split!.
+      tstep_s. eexists (Some (inr _)). split!. apply: steps_spec_step_end; [econs|] => /=? ->.
+      tstep_i. apply steps_impl_step_end => ???. invert_all @m_step. split!.
+      tstep_s. eexists (Some (inl _)). split!. apply: steps_spec_step_end; [econs|] => /=? ->.
+      tstep_i => ? <-.
+      tstep_i. eexists _, [ValNum _]. split!.
+      1: by apply: ucmra_discrete_update_valid.
+      1: done. 1: econs; [done|econs]. 1: done. 1: done.
+      apply: Hloop; [done|]. split!.
+      1: by apply: ucmra_discrete_update_valid.
+    + destruct i as [? []]; simplify_eq/=.
+      tstep_s. eexists (Some _). split!.
+      apply: steps_spec_step_end; [econs|]=> /=??. destruct_all?; simplify_eq/=.
+      tstep_s. eexists None. apply: steps_spec_step_end; [econs|]=> /=??. destruct_all?; simplify_eq/=.
+      destruct vs as [|v ?]; decompose_Forall_hyps. destruct v => //; simplify_eq/=.
+      tend. split!.
+      tstep_i. apply: steps_impl_step_end => ???. invert_all @m_step. split!.
+      tstep_i. apply: steps_impl_step_end => ???. invert_all @m_step. split!.
+      tstep_s. eexists (Some (inr _)). split!.
+      apply: steps_spec_step_end; [econs|]=> /=? ->.
+      tstep_i. apply: steps_impl_step_end => ???. invert_all @m_step.
+Qed.
+
+Lemma imp_heap_bij_trefines_implies_ctx_refines fnsi fnss :
+  dom (gset _) fnsi = dom (gset _) fnss →
+  trefines (MS imp_module (initial_imp_state fnsi))
+           (MS (imp_heap_bij imp_module) (initial_imp_heap_bij_state imp_module (initial_imp_state fnss))) →
+  imp_ctx_refines fnsi fnss.
+Proof.
+  move => Hdom Href C. rewrite /imp_link map_difference_union_r (map_difference_union_r fnss).
+  etrans; [|apply imp_heap_bij_imp_closed].
+  apply mod_seq_map_trefines. { apply _. } { apply _. }
+  etrans. { apply imp_link_refines_prod. apply map_disjoint_difference_r'. }
+  etrans. { apply: imp_prod_trefines. 1: done. 1: apply imp_heap_bij_imp_refl. }
+  etrans. { apply imp_heap_bij_combine; apply _. }
+  apply: mod_prepost_trefines.
+  etrans. 2: { apply imp_prod_refines_link. apply map_disjoint_difference_r'. }
+  rewrite !dom_difference_L Hdom.
+  erewrite map_difference_eq_dom_L => //.
+  apply _.
+Qed.
+
+Module imp_heap_bij_example.
+
+Local Open Scope Z_scope.
+
+Definition bij_alloc : fndef := {|
+  fd_args := [];
+  fd_body := (LetE "tmp" (Alloc (Val 1))
+             (LetE "_" (Store (Var "tmp") (Val 1))
+             (LetE "_" (Call "ext" [])
+             (LetE "res" (Load (Var "tmp"))
+             (LetE "_" (Free (Var "tmp"))
+             (Var "res"))))));
+  fd_static := I;
+|}.
+
+Definition bij_alloc_opt : fndef := {|
+  fd_args := [];
+  fd_body := (LetE "_" (Call "ext" [])
+             (Val 1));
+  fd_static := I;
+|}.
+
+Lemma bij_alloc_opt_refines :
+  trefines (MS imp_module (initial_imp_state (<["f" := bij_alloc_opt]> ∅)))
+           (MS (imp_heap_bij imp_module) (initial_imp_heap_bij_state imp_module
+                                            (initial_imp_state (<["f" := bij_alloc]> ∅)))).
+Proof.
+  pose (R := λ (b : bool) (r1 r2 : heap_bijUR), r1 ≼ r2).
+  apply: (imp_prepost_proof R); unfold R in *.
+  (* { constructor. { move => [??]. naive_solver. } *)
+  (*   { move => [??] [??] [??] [??] [??]. split; [by etrans|]. etrans; [done|]. *)
+  (*     by apply: heap_preserved_mono. } } *)
+  { move => [??] [??]. naive_solver. }
+  move => n K1 K2 f fn1 vs1 h0 r0 ?.
+  rewrite !lookup_insert_Some => ?; destruct_all?; simplify_map_eq/=.
+  move => bij1 ? h1 *. split!. move => ?. split!; [solve_length|].
+  move => Hcall Hret.
+  pose (l := (heap_fresh (dom _ (hb_bij bij1)) h1)).
+  have Hf := heap_fresh_not_in (dom _ (hb_bij bij1)) h1.
+  tstep_s. eexists l. split!. { apply heap_fresh_is_fresh. }
+  move => *; simplify_eq.
+  tstep_s. tstep_s. move => ? [<-] ?.
+  tstep_s.
+  apply: (Hcall _ _ ([LetECtx _ _]) ([LetECtx _ _])); [done|..].
+  1, 2: by simplify_map_eq. 1,2: by econs.
+  eexists (heap_bij_update_const l.1 _ bij1), [].
+  split!.
+  { rewrite -!assoc. etrans.
+    { apply cmra_update_op; [|done]. apply (heap_bij_alloc_const _ l.1). set_solver. }
+    rewrite -assoc. apply cmra_update_op; [done|].
+    rewrite comm -assoc. done. }
+  { etrans; [apply hb_shared_provs_update_const|]. done. }
+  { econs. }
+  { apply: heap_in_bij_update_r; [|move => *; simplify_map_eq].
+    apply: heap_in_bij_alloc_r; [|move => *; simplify_map_eq].
+    apply: heap_in_bij_mono_bij; [done|]. move => ?? /=/lookup_insert_Some?. naive_solver. }
+  { apply heap_preserved_update_const.
+    apply heap_preserved_update; [|move => *; simplify_map_eq].
+    apply heap_preserved_alloc; [|move => *; simplify_map_eq].
+    apply: heap_preserved_mono; [done|]. move => ?? /=/lookup_delete_Some?. naive_solver. }
+  { apply cmra_included_l. }
+  move => ? h2 r2 ? bij3 ? h3 *. decompose_Forall_hyps.
+  split!.
+  tstep_i.
+  tstep_s.
+  tstep_s. move => ?? [<-] /heap_preserved_lookup_r Hlookup.
+  eassert (hb_bij bij3 !! l.1 = Some (HBConstant _)). {
+    apply heap_bij_const_lookup. apply: cmra_valid_included; [done|].
+    rewrite -assoc. apply cmra_mono_l. apply cmra_included_op_r. etrans; [|done].
+    apply cmra_included_r.
+  }
+  efeed pose proof Hlookup as Hlookup'; [done..|].
+  simplify_map_eq.
+  tstep_s.
+  tstep_s => *. simplify_eq.
+  tstep_s.
+  apply: Hret; [done|].
+  eexists (heap_bij_update_const _ _ _), [ValNum 1]. split!.
+  { etrans. { by apply: cmra_update_op; [|by apply cmra_update_included]. }
+    rewrite assoc comm !assoc.
+    apply: cmra_update_op; [|done]. apply: cmra_update_op; [|done].
+    rewrite comm. etrans; [apply heap_bij_frag_update_const|]. apply cmra_update_op_l. }
+  all: split!.
+  { etrans; [apply hb_shared_provs_update_const|]. done. }
+  1: by econs.
+  { apply heap_in_bij_free_r. {
+      apply: heap_in_bij_mono_bij; [done|].
+      move => /=?? /lookup_insert_Some. naive_solver. }
+    move => ??. simplify_map_eq. }
+  { apply heap_preserved_update_const.
+    apply: heap_preserved_free; [ |move => *; simplify_map_eq].
+    apply: heap_preserved_mono; [done|]. move => ?? /lookup_delete_Some; naive_solver.
+  }
+Qed.
+
+Lemma bij_alloc_ctx_refines :
+  imp_ctx_refines (<["f" := bij_alloc_opt]> ∅) (<["f" := bij_alloc]> ∅).
+Proof.
+  apply: imp_heap_bij_trefines_implies_ctx_refines. { set_solver. }
+  apply bij_alloc_opt_refines.
+Qed.
+End imp_heap_bij_example.
