theories/imp_to_asm_examples.v
@@ -4,6 +4,7 @@ Require Import refframe.filter.
 Require Import refframe.product.
 Require Import refframe.seq_product.
 Require Import refframe.proof_techniques.
+Require Import refframe.prepost.
 Require Import refframe.imp.
 Require Import refframe.asm.
 Require Import refframe.imp_to_asm.
@@ -215,12 +216,41 @@ Proof.
   apply lookup_lookup_total; simplify_map_eq'.
 Qed.
 
-(* TODO: prove the following: *)
-(* Lemma imp_add_refines_imp_add' : *)
-(*   trefines (MS imp_module (initial_imp_state full_imp_add_prog)) *)
-(*            (MS imp_module (initial_imp_state full_imp_add_prog')). *)
-(* Proof. *)
+(*
+The following does not actually hold since the allocation adds a new provenance to h_heap provs
 
+Lemma imp_add_refines_imp_add' :
+  trefines (MS imp_module (initial_imp_state full_imp_add_prog))
+           (MS (mod_prepost prepost_id prepost_id imp_module)
+               (SMFilter, initial_imp_state full_imp_add_prog', (PPOutside, tt))).
+Proof.
+  pose (R := λ (b : bool) (r1 r2 : unit), True).
+  apply: (imp_prepost_proof R); unfold R in *.
+  { done. }
+  unfold full_imp_add_prog. move => n K1 K2 f fn1 vs1 h0 r0 ?.
+  rewrite lookup_union_Some_raw !lookup_insert_Some => ?; destruct_all?; simplify_map_eq/=.
+  all: split! => ?; split! => Hcall Hret.
+  - destruct vs1 as [|? [|??]] => //. by tstep_s.
+  - destruct vs1 => //.
+    tstep_i => *. split!.
+    tstep_i.
+    tstep_i. split!. { by apply heap_alive_alloc. }
+    tstep_i.
+    tstep_i. simplify_map_eq. eexists _.
+    split. { rewrite shift_loc_0. by simplify_map_eq. }
+    tstep_i.
+    tstep_i. split!. { apply heap_alive_update. by apply heap_alive_alloc. }
+    tstep_i.
+    change (imp.Call "add" [Val 1; Val 1]) with (imp.Call "add" (Val <$> [ValNum 1; ValNum 1])).
+    tstep_i. simplify_map_eq. split; [|naive_solver].
+    move => ??. simplify_map_eq. split!.
+    tstep_i.
+    apply Hret; [done|]. split!.
+    f_equal.
+    f_equal.
+    by rewrite heap_free_update // heap_free_alloc // heap_free_fresh.
+Qed.
+*)
 
 Lemma full_add_stack :
   trefines (MS asm_module (initial_asm_state full_asm_add))
@@ -252,6 +282,12 @@ Proof.
     unfold imp_add_prog, imp_add_client_prog. eauto with map_disjoint.
   }
   done.
+  (* etrans. { *)
+  (*   apply: imp_to_asm_trefines. *)
+  (*   apply: imp_add_refines_imp_add'. *)
+  (* } *)
+  (* etrans. { apply: prepost_id_l. } *)
+  (* done. *)
 Qed.
 
 (* TODO: an interesting example would be to prove
